external/Goose/github_com/mit_pdos/go_mvcc/examples.v
@@ -4,146 +4,25 @@ From Goose Require github_com.mit_pdos.go_mvcc.txn.
 
 From Perennial.goose_lang Require Import ffi.grove_prelude.
 
-(* counter.go *)
-
-Definition fetch: val :=
-  rec: "fetch" "txn" "p" :=
-    let: ("v", <>) := txn.Txn__Get "txn" #0 in
-    "p" <-[uint64T] "v";;
+Definition hello: val :=
+  rec: "hello" "txn" :=
+    txn.Txn__Put "txn" #0 #(str"hello");;
+    txn.Txn__Get "txn" #0;;
+    txn.Txn__Delete "txn" #0;;
     #true.
 
-Definition Fetch: val :=
-  rec: "Fetch" "t" :=
-    let: "n" := ref (zero_val uint64T) in
-    let: "body" := (λ: "txn",
-      fetch "txn" "n"
+Definition Hello: val :=
+  rec: "Hello" "txno" :=
+    let: "body" := (λ: "txni",
+      hello "txni"
       ) in
-    txn.Txn__DoTxn "t" "body";;
-    ![uint64T] "n".
-
-Definition increment: val :=
-  rec: "increment" "txn" "p" :=
-    let: ("v", <>) := txn.Txn__Get "txn" #0 in
-    "p" <-[uint64T] "v";;
-    (if: ("v" = #18446744073709551615)
-    then #false
-    else
-      txn.Txn__Put "txn" #0 ("v" + #1);;
-      #true).
-
-Definition Increment: val :=
-  rec: "Increment" "t" :=
-    let: "n" := ref (zero_val uint64T) in
-    let: "body" := (λ: "txn",
-      increment "txn" "n"
-      ) in
-    let: "ok" := txn.Txn__DoTxn "t" "body" in
-    (![uint64T] "n", "ok").
-
-Definition decrement: val :=
-  rec: "decrement" "txn" "p" :=
-    let: ("v", <>) := txn.Txn__Get "txn" #0 in
-    "p" <-[uint64T] "v";;
-    (if: ("v" = #0)
-    then #false
-    else
-      txn.Txn__Put "txn" #0 ("v" - #1);;
-      #true).
-
-Definition Decrement: val :=
-  rec: "Decrement" "t" :=
-    let: "n" := ref (zero_val uint64T) in
-    let: "body" := (λ: "txn",
-      decrement "txn" "n"
-      ) in
-    let: "ok" := txn.Txn__DoTxn "t" "body" in
-    (![uint64T] "n", "ok").
-
-Definition InitializeCounterData: val :=
-  rec: "InitializeCounterData" "mgr" :=
-    let: "body" := (λ: "txn",
-      txn.Txn__Put "txn" #0 #0;;
-      #true
-      ) in
-    let: "t" := txn.TxnMgr__New "mgr" in
-    Skip;;
-    (for: (λ: <>, ~ (txn.Txn__DoTxn "t" "body")); (λ: <>, Skip) := λ: <>,
-      Continue);;
+    txn.Txn__DoTxn "txno" "body";;
     #().
 
-Definition InitCounter: val :=
-  rec: "InitCounter" <> :=
-    let: "mgr" := txn.MkTxnMgr #() in
-    InitializeCounterData "mgr";;
-    "mgr".
-
-Definition CallIncrement: val :=
-  rec: "CallIncrement" "mgr" :=
-    let: "txn" := txn.TxnMgr__New "mgr" in
-    Increment "txn";;
+Definition CallHello: val :=
+  rec: "CallHello" <> :=
+    let: "db" := txn.MkTxnMgr #() in
+    txn.TxnMgr__ActivateGC "db";;
+    let: "txn" := txn.TxnMgr__New "db" in
+    Hello "txn";;
     #().
-
-Definition CallIncrementFetch: val :=
-  rec: "CallIncrementFetch" "mgr" :=
-    let: "txn" := txn.TxnMgr__New "mgr" in
-    let: ("n1", "ok1") := Increment "txn" in
-    (if: ~ "ok1"
-    then #()
-    else
-      let: "n2" := Fetch "txn" in
-      control.impl.Assert ("n1" < "n2");;
-      #()).
-
-Definition CallDecrement: val :=
-  rec: "CallDecrement" "mgr" :=
-    let: "txn" := txn.TxnMgr__New "mgr" in
-    Decrement "txn";;
-    #().
-
-(* rsvkey.go *)
-
-Definition WriteReservedKeySeq: val :=
-  rec: "WriteReservedKeySeq" "txn" "v" :=
-    txn.Txn__Put "txn" #0 "v";;
-    #true.
-
-Definition WriteReservedKey: val :=
-  rec: "WriteReservedKey" "t" "v" :=
-    let: "body" := (λ: "txn",
-      WriteReservedKeySeq "txn" "v"
-      ) in
-    txn.Txn__DoTxn "t" "body".
-
-Definition WriteFreeKeySeq: val :=
-  rec: "WriteFreeKeySeq" "txn" "v" :=
-    txn.Txn__Put "txn" #1 "v";;
-    #true.
-
-Definition WriteFreeKey: val :=
-  rec: "WriteFreeKey" "t" "v" :=
-    let: "body" := (λ: "txn",
-      WriteFreeKeySeq "txn" "v"
-      ) in
-    txn.Txn__DoTxn "t" "body".
-
-Definition InitializeData: val :=
-  rec: "InitializeData" "mgr" :=
-    #().
-
-Definition InitExample: val :=
-  rec: "InitExample" <> :=
-    let: "mgr" := txn.MkTxnMgr #() in
-    InitializeData "mgr";;
-    "mgr".
-
-Definition WriteReservedKeyExample: val :=
-  rec: "WriteReservedKeyExample" "mgr" "v" :=
-    let: "txn" := txn.TxnMgr__New "mgr" in
-    let: "ok" := WriteReservedKey "txn" "v" in
-    "ok".
-
-Definition WriteFreeKeyExample: val :=
-  rec: "WriteFreeKeyExample" "mgr" "v" :=
-    let: "txn" := txn.TxnMgr__New "mgr" in
-    let: "ok" := WriteFreeKey "txn" "v" in
-    "ok".
