src/program_proof/mvcc/examples_hello.v
@@ -1,0 +1,155 @@
+(* [mono_nat] must go first otherwise the default scope becomes nat. *)
+From iris.base_logic Require Import mono_nat.
+From Perennial.program_proof Require Import
+     mvcc_prelude mvcc_ghost mvcc_inv
+     txnmgr_repr txnmgr_mk txnmgr_new txnmgr_activate_gc
+     txn_repr txn_get txn_put txn_delete txn_do_txn.
+From Goose.github_com.mit_pdos.go_mvcc Require Import examples.
+
+Section program.
+Context `{!heapGS Σ, !mvcc_ghostG Σ}.
+
+Definition P_Hello (r : dbmap) := ∃ v, r = {[ (U64 0) := v ]}.
+Definition Q_Hello (r w : dbmap) := w = {[ (U64 0) := Nil ]}.
+
+Theorem wp_hello txn tid r γ τ :
+  {{{ own_txn txn tid r γ τ ∗ ⌜P_Hello r⌝ ∗ txnmap_ptstos τ r }}}
+    hello #txn
+  {{{ (ok : bool), RET #ok;
+      own_txn txn tid r γ τ ∗
+      if ok
+      then ∃ w, ⌜Q_Hello r w ∧ dom r = dom w⌝ ∗
+                txnmap_ptstos τ w
+      else True
+  }}}.
+Proof.
+  iIntros (Φ) "(Htxn & %HP & Hpt) HΦ".
+  wp_call.
+  unfold txnmap_ptstos.
+  destruct HP as [v HP].
+  rewrite HP.
+  rewrite big_sepM_singleton.
+
+  (***********************************************************)
+  (* txn.Put(0, "hello")                                     *)
+  (* txn.Get(0)                                              *)
+  (* txn.Delete(0)                                           *)
+  (* return true                                             *)
+  (***********************************************************)
+  wp_apply (wp_txn__Put with "[$Htxn $Hpt]").
+  iIntros "[Htxn Hpt]".
+  wp_apply (wp_txn__Get with "[$Htxn $Hpt]").
+  iIntros (u found) "[Htxn [Hpt %Hu]]".
+  wp_pures.
+  wp_apply (wp_txn__Delete with "[$Htxn $Hpt]").
+  iIntros (ok) "[Htxn Hpt]".
+  wp_pures.
+  iApply "HΦ".
+  iFrame.
+  iModIntro.
+  iExists {[ (U64 0) := Nil ]}.
+  rewrite big_sepM_singleton.
+  iFrame.
+  iPureIntro.
+  unfold Q_Hello.
+  set_solver.
+Qed.
+
+Theorem wp_Hello (txn : loc) γ :
+  ⊢ {{{ own_txn_uninit txn γ }}}
+    <<< ∀∀ (v : dbval), dbmap_ptsto γ (U64 0) 1 v >>>
+      Hello #txn @ ↑mvccN
+    <<< ∃∃ (ok : bool), if ok then dbmap_ptsto γ (U64 0) 1 Nil else dbmap_ptsto γ (U64 0) 1 v >>>
+    {{{ RET #(); own_txn_uninit txn γ }}}.
+Proof.
+  iIntros "!>".
+  iIntros (Φ) "Htxn HAU".
+  wp_call.
+
+  (***********************************************************)
+  (* body := func(txn *txn.Txn) bool {                       *)
+  (*     return hello(txn)                                   *)
+  (* }                                                       *)
+  (* ok := t.DoTxn(body)                                     *)
+  (***********************************************************)
+  wp_apply (wp_txn__DoTxn_xres _ _ P_Hello Q_Hello with "[$Htxn]").
+  { unfold Q_Hello. apply _. }
+  { unfold spec_body_xres.
+    clear Φ.
+    iIntros (tid r τ Φ) "(Htxn & %HP & Htxnpt) HΦ".
+    wp_pures.
+    wp_apply (wp_hello with "[$Htxn $Htxnpt]"); first done.
+    iApply "HΦ".
+  }
+  iMod "HAU".
+  iModIntro.
+  iDestruct "HAU" as (v) "[Hdbpt HAU]".
+  iExists {[ (U64 0) := v ]}.
+  iSplitL "Hdbpt".
+  { unfold dbmap_ptstos.
+    rewrite big_sepM_singleton.
+    iFrame.
+    iPureIntro.
+    unfold P_Hello.
+    by eauto.
+  }
+  iIntros (ok w) "Hdbpt".
+  iFrame.
+  destruct ok eqn:E.
+  { (* Case COMMIT. *)
+    unfold Q_Hello.
+    iDestruct "Hdbpt" as "[%HQ Hdbpt]".
+    rewrite HQ /dbmap_ptstos big_sepM_singleton.
+    iMod ("HAU" $! true with "Hdbpt") as "HΦ".
+    iIntros "!> Htxn".
+    wp_pures.
+    by iApply "HΦ".
+  }
+  { (* Case ABORT. *)
+    rewrite /dbmap_ptstos big_sepM_singleton.
+    iMod ("HAU" $! false with "Hdbpt") as "HΦ".
+    iIntros "!> Htxn".
+    wp_pures.
+    by iApply "HΦ".
+  } 
+Qed.
+
+Theorem wp_CallHello :
+  {{{ True }}}
+    CallHello #()
+  {{{ RET #(); True }}}.
+Proof using heapGS0 mvcc_ghostG0 Σ.
+  iIntros (Φ) "_ HΦ".
+  wp_call.
+
+  (***********************************************************)
+  (* db := txn.MkTxnMgr()                                    *)
+  (* db.ActivateGC()                                         *)
+  (* txn := db.New()                                         *)
+  (* Hello(txn)                                              *)
+  (***********************************************************)
+  wp_apply wp_MkTxnMgr.
+  iIntros (γ mgr) "[#Hmgr Hdbpts]".
+  wp_pures.
+  wp_apply (wp_txnMgr__ActivateGC with "Hmgr").
+  wp_pures.
+  wp_apply (wp_txnMgr__New with "Hmgr").
+  iIntros (txn) "Htxn".
+  wp_pures.
+  wp_apply (wp_Hello with "Htxn").
+  iApply ncfupd_mask_intro; first set_solver.
+  iIntros "Hmask".
+  iDestruct (big_sepM_lookup _ _ (U64 0) with "Hdbpts") as "Hdbpt".
+  { rewrite lookup_gset_to_gmap_Some.
+    split; [set_solver | reflexivity].
+  }
+  iExists Nil.
+  iFrame.
+  iIntros (ok) "Hdbpt".
+  iMod "Hmask" as "_".
+  iIntros "!> Htxn".
+  wp_pures.
+  by iApply "HΦ".
+Qed.
+
+End program.
